chore: add globals invariant

theories/Subset.v
@@ -2,7 +2,7 @@ From MetaCoq.Common Require Import Kernames.
 From MetaCoq.Utils Require Import utils.
 From MetaCoq.Erasure.Typed Require Import Utils ResultMonad.
 From MetaCoq.Erasure.Typed Require Import Annotations WcbvEvalAux.
-From MetaCoq.Erasure Require Import EAst ECSubst ELiftSubst.
+From MetaCoq.Erasure Require Import EAst ECSubst EGlobalEnv ELiftSubst.
 From MetaCoq.Erasure.Typed Require Import ExAst.
 
 From VTL Require Import PIR BigStepPIR Translation Utils.
@@ -11,47 +11,48 @@ Existing Instance EWcbvEval.default_wcbv_flags.
 
 From Coq Require Import Strings.String Lia.
 
-Inductive InSubset (Γ : list string) : EAst.term -> Prop :=
-  | S_tBox : InSubset Γ tBox
+Inductive InSubset (eΣ : global_env) (Γ : list string) : EAst.term -> Prop :=
+  | S_tBox : InSubset eΣ Γ tBox
   | S_tRel : forall n res,
     nth_error Γ n = Some res ->
-    InSubset Γ (tRel n)
+    InSubset eΣ Γ (tRel n)
   | S_tLambda : forall x x' b,
-    InSubset (x' :: Γ) b ->
-    InSubset Γ (tLambda x b)
+    InSubset eΣ (x' :: Γ) b ->
+    InSubset eΣ Γ (tLambda x b)
   | S_tLet : forall x x' br b,
-    InSubset Γ br ->
-    InSubset (x' :: Γ) b ->
-    InSubset Γ (tLetIn x br b)
+    InSubset eΣ Γ br ->
+    InSubset eΣ (x' :: Γ) b ->
+    InSubset eΣ Γ (tLetIn x br b)
   | S_tApp : forall f a,
-    InSubset Γ f ->
-    InSubset Γ a ->
-    InSubset Γ (tApp f a)
-  | S_tConst : forall eΣ kn cb,
-    lookup_constant_body eΣ kn = Some cb ->
-    InSubset [] cb ->
-    (* translate_env remap_env eΣ ann_env = Ok Σ' ->
-    lookup_entry Σ' kn = Some (kn, kn', br) -> *)
-    InSubset Γ (tConst kn)
+    InSubset eΣ Γ f ->
+    InSubset eΣ Γ a ->
+    InSubset eΣ Γ (tApp f a)
+  | S_tConst : forall eΣ' kn decl cb,
+    declared_constant (trans_env eΣ) kn decl ->
+    decl.(EAst.cst_body) = Some cb ->
+    InSubset eΣ' [] cb ->
+    InSubset eΣ Γ (tConst kn)
 .
 
-Definition declared_constant (eΣ : global_env) kn c : Prop :=
-  lookup_env eΣ kn = Some (ConstantDecl c).
+(* Definition declared_constant (eΣ : global_env) kn c : Prop :=
+  lookup_env eΣ kn = Some (ConstantDecl c). *)
 
 Definition all_in_subset eΣ :=
-  forall c decl, declared_constant eΣ c decl -> exists t, cst_body decl = Some t /\ InSubset [] t.
+  forall c decl, 
+    declared_constant (trans_env eΣ) c decl -> 
+    exists t, EAst.cst_body decl = Some t /\ InSubset eΣ [] t.
 
 Inductive ProgramInSubset (eΣ : global_env) (init : kername) : Prop :=
   | PS_Constants :
     all_in_subset eΣ ->
-    (exists t, lookup_constant_body eΣ init = Some t) ->
+    (exists t, declared_constant (trans_env eΣ) init t) ->
     ProgramInSubset eΣ init.
 
-Lemma mkApps_in_subset : forall Γ us f,
-  InSubset Γ (mkApps f us) ->
-  InSubset Γ f /\ (forall a, In a us -> InSubset Γ a).
+Lemma mkApps_in_subset : forall eΣ Γ us f,
+  InSubset eΣ Γ (mkApps f us) ->
+  InSubset eΣ Γ f /\ (forall a, In a us -> InSubset eΣ Γ a).
 Proof.
-  intros Γ us. induction us.
+  intros eΣ Γ us. induction us.
   - intros. simpl in *. auto.
   - intros. simpl in H. specialize (IHus (tApp f a)).
     apply IHus in H. destruct H as [Hf Hus]. 
@@ -63,13 +64,13 @@ Proof.
       * apply Hus. assumption.
 Qed.
 
-Lemma subset_weaken : forall Γ x t,
-  InSubset Γ t ->
-  InSubset (Γ ++ [x]) t.
+Lemma subset_weaken : forall eΣ Γ x t,
+  InSubset eΣ Γ t ->
+  InSubset eΣ (Γ ++ [x]) t.
 Proof.
-  intros Γ x t sub. induction sub.
+  intros eΣ Γ x t sub. induction sub.
   - constructor.
-  - apply (S_tRel (Γ ++ [x]) n res). 
+  - apply (S_tRel eΣ (Γ ++ [x]) n res). 
     apply nth_error_Some_length in H as Hl.
     rewrite (nth_error_app1 Γ [x] Hl). assumption.
   - eapply S_tLambda. apply IHsub.
@@ -78,13 +79,13 @@ Proof.
   - eapply S_tConst; eassumption.
 Qed.
 
-Lemma subset_weaken_many : forall Γ1 Γ2 t,
-  InSubset Γ1 t ->
-  InSubset (Γ1 ++ Γ2) t.
+Lemma subset_weaken_many : forall eΣ Γ1 Γ2 t,
+  InSubset eΣ Γ1 t ->
+  InSubset eΣ (Γ1 ++ Γ2) t.
 Proof.
-  intros Γ1 Γ2 t sub. induction sub.
+  intros eΣ Γ1 Γ2 t sub. induction sub.
   - constructor.
-  - apply (S_tRel (Γ ++ Γ2) n res). 
+  - apply (S_tRel eΣ (Γ ++ Γ2) n res). 
     apply nth_error_Some_length in H as Hl.
     rewrite (nth_error_app1 Γ Γ2 Hl). assumption.
   - eapply S_tLambda. apply IHsub.
@@ -93,27 +94,27 @@ Proof.
   - eapply S_tConst; eassumption.
 Qed.
 
-Lemma csubst_in_sub' : forall (Γ1 Γ2 : list string) x v b,
-  InSubset [] v ->
-  InSubset (Γ1 ++ x :: Γ2) b ->
-  InSubset (Γ1 ++ Γ2) (csubst v #|Γ1| b).
+Lemma csubst_in_sub' : forall eΣ Γ1 Γ2 x v b,
+  InSubset eΣ [] v ->
+  InSubset eΣ (Γ1 ++ x :: Γ2) b ->
+  InSubset eΣ (Γ1 ++ Γ2) (csubst v #|Γ1| b).
 Proof.
-  intros Γ1 Γ2 x v b sub_v.
+  intros eΣ Γ1 Γ2 x v b sub_v.
   revert Γ1 x; induction b; 
   intros Γ1 x sub_b; inversion sub_b.
   remember (Γ1 ++ x :: Γ2) as Γ.
   - simpl. constructor.
   - simpl. subst. destruct (#|Γ1| ?= n) eqn:Ec.
-    + apply (subset_weaken_many [] (Γ1 ++ Γ2) v) in sub_v.
+    + apply (subset_weaken_many eΣ [] (Γ1 ++ Γ2) v) in sub_v.
       apply sub_v.
     + apply Nat.compare_lt_iff in Ec.
       apply nth_error_Some_length, length_pred_middle in H0.
       apply nth_error_Some_value in H0. destruct H0.
-      apply (S_tRel (Γ1 ++ Γ2) (Nat.pred n) x0 H). assumption.
+      apply (S_tRel eΣ (Γ1 ++ Γ2) (Nat.pred n) x0 H). assumption.
     + apply Nat.compare_gt_iff in Ec.
       apply length_extend with (l2 := Γ2) in Ec.
       apply nth_error_Some_value in Ec. destruct Ec.
-      apply (S_tRel (Γ1 ++ Γ2) n x0 H).
+      apply (S_tRel eΣ (Γ1 ++ Γ2) n x0 H).
   - simpl. econstructor.
     apply (IHb (x' :: Γ1) x). apply H0.
   - simpl. econstructor.
@@ -125,30 +126,29 @@ Proof.
   - eapply S_tConst; eassumption.
 Qed.
 
-Lemma csubst_in_sub : forall (Γ : list string) x v b,
-  InSubset [] v ->
-  InSubset (Γ ++ [x]) b ->
-  InSubset Γ (csubst v #|Γ| b).
+Lemma csubst_in_sub : forall eΣ (Γ : list string) x v b,
+  InSubset eΣ [] v ->
+  InSubset eΣ (Γ ++ [x]) b ->
+  InSubset eΣ Γ (csubst v #|Γ| b).
 Proof.
-  intros. assert (forall t, InSubset Γ t = InSubset (Γ ++ []) t) by (rewrite app_nil_r; reflexivity).
-  rewrite H1. eapply (csubst_in_sub' Γ [] x v b); assumption.
+  intros. assert (forall t, InSubset eΣ Γ t = InSubset eΣ (Γ ++ []) t) by (rewrite app_nil_r; reflexivity).
+  rewrite H1. eapply (csubst_in_sub' eΣ Γ [] x v b); assumption.
 Qed.
 
-(* Lemma everything in global env is in subset*)
-Lemma val_in_sub : forall Σ Γ t v,
-  Σ e⊢ t ⇓ v ->
-  InSubset Γ t ->
-  InSubset Γ v.
+Lemma val_in_sub : forall eΣ Γ t v,
+  (trans_env eΣ) e⊢ t ⇓ v ->
+  InSubset eΣ Γ t ->
+  InSubset eΣ Γ v.
 Proof.
-  intros Σ Γ t v ev. revert Γ. induction ev; intros Γ sub; inversion sub; subst.
+  intros eΣ Γ t v ev. revert Γ. induction ev; intros Γ sub; inversion sub; subst.
   - constructor.
   - specialize (IHev1 Γ H1). invs IHev1.
     specialize (IHev2 Γ H2). apply IHev3.
-    eapply (csubst_in_sub' [] Γ).
+    eapply (csubst_in_sub' eΣ [] Γ).
     admit. apply H0.
   - specialize (IHev1 Γ H1).
     apply IHev2.
-    eapply (csubst_in_sub' [] Γ).
+    eapply (csubst_in_sub' eΣ [] Γ).
     admit. apply H3.
   - apply IHev1 in H1. apply mkApps_in_subset in H1 as [Hf _]. inversion Hf.
   - apply IHev1 in H1. apply mkApps_in_subset in H1 as [Hf _]. inversion Hf.
@@ -162,9 +162,9 @@ Proof.
   - assumption.
 Admitted.
 
-Lemma tlt_in_sub : forall TT Σ' Γ t ann t',
+Lemma tlt_in_sub : forall TT eΣ Σ' Γ t ann t',
   translatesTo TT Σ' Γ t ann t' ->
-  InSubset Γ t.
+  InSubset eΣ Γ t.
 Proof.
   intros. induction H; subst.
   - constructor.
@@ -176,11 +176,11 @@ Proof.
 Admitted.
 
 (* notion of typablility under the remapping *)
-Lemma subset_is_translatable : forall TT Σ' Γ t,
-  InSubset Γ t ->
+Lemma subset_is_translatable : forall TT eΣ Σ' Γ t,
+  InSubset eΣ Γ t ->
   exists ann t', translate_term TT Σ' Γ t ann = Some t'.
 Proof.
-  intros TT Σ' Γ t sub. 
+  intros TT eΣ Σ' Γ t sub. 
   induction sub; subst.
   - eexists _, _. constructor.
   - eexists. exists (Var res).
@@ -243,20 +243,24 @@ Definition subset_env_flags :=
 
 Local Existing Instance subset_env_flags.
 
-Lemma lookup_constant_env_ex_env : forall Σ kn cb cb',
-  EGlobalEnv.declared_constant (trans_env Σ) kn cb ->
-  lookup_constant_body Σ kn = Some cb'.
+Lemma lookup_env_context : forall eΣ kn c,
+  EGlobalEnv.lookup_env (trans_env eΣ) kn = Some (EAst.ConstantDecl c) ->
+  exists c', lookup_constant eΣ kn = Some c'.
 Proof.
-  intros Σ kn cb cb' Hl.
-  induction Σ.
+  (* intros eΣ kn cb cb' t [Hl Hsome].
+  induction eΣ.
   - inversion Hl.
   - destruct a as [[kn' deps] decl].
-    unfold EGlobalEnv.declared_constant in Hl.
-    rewrite lookup_env_find in Hl. simpl in Hl.
     destruct (kn == kn') eqn:Heq.
-    + inversion Hl.
-      unfold lookup_constant_body, lookup_constant, lookup_env.
-      simpl. rewrite Heq. simpl.
+    + apply ReflectEq.eqb_eq in Heq. subst.
+      unfold EGlobalEnv.lookup_constant, EGlobalEnv.lookup_env in Hl. simpl in Hl.
+      unfold lookup_constant_body, lookup_constant, lookup_env. *)
+      (* simpl. rewrite ReflectEq.eqb_refl. rewrite ReflectEq.eqb_refl in Hl.
+      simpl in Hl. simpl. destruct cb. destruct cst_body; try discriminate.
+      destruct decl; try discriminate.
+      * simpl. inversion Hl. inversion Hsome. subst. destruct c. inversion Hl. admit.
+      * inversion Hl. destruct o; try discriminate. inversion H0. subst. simpl in Hl.
+        destruct t; try discriminate. *)
 Admitted.
 
 (* lookup_env_find *)
@@ -269,14 +273,18 @@ Proof.
   induction eΣ.
   - inversion Hinit.
   - destruct a as [[kn deps] decl].
-    constructor.
-    + admit.
-    + eexists. now eapply lookup_constant_env_ex_env.
+    inversion Hinit.
+    destruct (init == kn) eqn:Heq.
+    + apply ReflectEq.eqb_eq in Heq. subst.
+      inversion Hinit. rewrite ReflectEq.eqb_refl in H1.
+      inversion H1. cbn. inversion Hwf. subst.
+      constructor. hnf. intros. inversion H. inversion H6.
+      subst. eexists.
 Admitted.
 
 Lemma wellformed_implies_subset : forall eΣ Γ t,
   @wellformed subset_env_flags (trans_env eΣ) (List.length Γ) t ->
-  InSubset Γ t.
+  InSubset eΣ Γ t.
 Proof.
   intros eΣ Γ t. revert Γ.
   induction t; intros Γ Hwf; inversion Hwf.
@@ -284,19 +292,23 @@ Proof.
   - apply Nat.ltb_lt, nth_error_Some_value in H0.
     destruct H0. now eapply S_tRel.
   - pose (na' := gen_fresh_name na [] Γ).
-    apply (S_tLambda Γ na na'). apply IHt. 
+    apply (S_tLambda eΣ Γ na na'). apply IHt. 
     simpl. apply H0.
   - apply andb_true_iff in H0 as [Hwf_t1 Hwf_t2].
     pose (na' := gen_fresh_name na [] Γ).
-    apply (S_tLet Γ na na'). 
+    apply (S_tLet eΣ Γ na na'). 
     apply IHt1; assumption.
     apply IHt2; assumption.
   - apply andb_true_iff in H0 as [Hwf_t1 Hwf_t2].
-    apply (S_tApp Γ).
+    apply (S_tApp eΣ Γ).
     apply IHt1; assumption.
     apply IHt2; assumption.
   - destruct (EGlobalEnv.lookup_constant (trans_env eΣ) k) eqn:Hl; [|discriminate].
-    destruct eΣ; try discriminate. 
-    eapply S_tConst. admit. admit.
+    destruct eΣ; try discriminate. destruct p as [[k' deps] decl].
+    destruct (k == k') eqn:Heq.
+    + apply ReflectEq.eqb_eq in Heq. subst.
+      admit.
+    + econstructor. unfold EGlobalEnv.declared_constant. simpl. rewrite Heq.
+      admit. admit. admit.
   - destruct prim as [[]]; inversion Hwf.
 Admitted.
